some more work on typed compilation

SystemFD/Hs/HsTerm.lean
@@ -26,6 +26,10 @@ protected def HsTerm.repr : (a : HsTerm) -> (p : Nat) -> Std.Format
 instance HsTerm_repr : Repr HsTerm where
   reprPrec a p := HsTerm.repr a p
 
+notation:15 a " `@ " b => HsTerm.HsApp a b
+notation:15 "`λ[" a "]" b => HsTerm.HsLam a b
+prefix:max "#" => HsTerm.HsVar
+notation:15 "if " p " ← " s " then " i " else " e => HsTerm.HsIte p s i e
 
 namespace HsTerm
  @[simp]
@@ -36,90 +40,175 @@ namespace HsTerm
  | HsLet t1 t2 t3 => Term.size t1 + size t2 + size t3 + 1
  | HsIte t1 t2 t3 t4 => size t1 + size t2 + size t3 + size t4 + 1
  -- | HsType t => Term.size t
+
+  @[simp]
+  def neutral_form : HsTerm -> Option (Nat × List HsTerm)
+  | .HsVar x => .some (x, [])
+  | .HsApp f a => do
+    let (x, sp) <- neutral_form f
+    .some (x, sp ++ [a])
+  | _ => .none
 end HsTerm
 
 instance sizeOf_HsTerm : SizeOf HsTerm where
   sizeOf := HsTerm.size
 
+
+def HsValidHeadVariable (t : HsTerm) (test : Nat -> Bool) : Prop :=
+  ∃ x, .some x = HsTerm.neutral_form t ∧ test x.fst
+
 inductive HsJudgment : Ctx Term -> HsTerm -> Term -> Prop where
 | var :
   Judgment .wf Γ () ->
   (Γ d@ x).get_type = .some T ->
-  HsJudgment Γ (.HsVar x) T
+  HsJudgment Γ (#x) T
+--- Implicit arrow and ∀ introduction/elimination
+| implicitArrI :
+  HsJudgment (.empty :: Γ) t τ ->
+  Γ ⊢ e : π ->
+  HsJudgment Γ t (π -t> τ)
+| implicitArrE :
+  HsJudgment Γ t (π -t> τ) ->
+  Γ ⊢ e : π ->
+  HsJudgment Γ t (τ β[e])
+| implicitAllI :
+  HsJudgment (.kind A :: Γ) t τ ->
+  Γ ⊢ A : ★ ->
+  HsJudgment Γ t (∀[A] τ)
+| implicitAllE :
+  HsJudgment Γ t (∀[A] τ) ->
+  Γ ⊢ A : ★ ->
+  HsJudgment Γ t (τ β[A])
+-- Term typing
 | lam :
   Judgment .prf Γ (A, ★) ->
   Judgment .prf Γ (A -t> B, ★) ->
   HsJudgment (.type A :: Γ) t B ->
-  HsJudgment Γ (.HsLam A t) (A -t> B)
+  HsJudgment Γ (`λ[A] t) (A -t> B)
 | app :
   HsJudgment Γ t1 (A -t> B) ->
   HsJudgment Γ t2 A ->
   B' = B β[A] ->
-  HsJudgment Γ (.HsApp t1 t2) B'
+  HsJudgment Γ (t1 `@ t2) B'
 | letterm :
   HsJudgment Γ t1 A ->
   HsJudgment (.type A :: Γ) t2 ([S] B) ->
   HsJudgment Γ (.HsLet A t1 t2) B
--- TODO ite
--- | ite :
---   HsJudgment Γ t1 A ->
---   HsJudgment (.type A :: Γ) t2 ([S] B) ->
---   HsJudgment Γ (.HsLet A t1 t2) B
+| ite :
+  HsJudgment Γ t1 A ->
+  HsJudgment Γ t2 A ->
+  HsJudgment Γ t3 B ->
+  HsJudgment Γ t4 B' ->
+  HsJudgment Γ (HsTerm.HsIte t1 t2 t3 t4) B
 
 
 notation: 170 Γ:170 " ⊢s " t:170 " : " A:170 => HsJudgment Γ t A
 
-inductive Compile : {Γ : Ctx Term} -> {t : HsTerm} -> {τ : Term} -> Γ ⊢s t : τ -> Term -> Prop where
+inductive Compile : {Γ : Ctx Term} -> {τ : Term} -> (t : HsTerm) ->  Γ ⊢s t : τ -> Term -> Prop where
 | var :
+  ⊢ Γ ->
+  (Γ d@ i).get_type = .some τ ->
   (j1 : Γ ⊢s (.HsVar i) : τ) ->
-  Compile j1 (Term.var i)
+  Compile (.HsVar i) j1 (Term.var i)
 | app :
   (j1 : Γ ⊢s t1 : (τ' -t> τ)) ->
   (j2 : Γ ⊢s t2 : τ') ->
-  (j3 : Γ ⊢s (.HsApp t1 t2) : (τ β[t2'])) ->
-  Compile j1 t1' ->
-  Compile j2 t2' ->
-  Compile j3 (t1' `@ t2')
+  (j3 : Γ ⊢s (t1 `@ t2) : (τ β[t2'])) ->
+  Compile t1 j1 t1' ->
+  Compile t2 j2 t2' ->
+  Compile (t1 `@ t2) j3 (t1' `@ t2')
 | appev :
   (j1 : Γ ⊢s t1 : (π -t> τ)) -> -- Γ ⊢ t1 : F a => τ
   (ValidHeadVariable π Γ.is_opent) ->
   Γ ⊢ e : π ->
-  Compile j1 t1' ->
+  Compile t1 j1 t1' ->
   (j2 : Γ ⊢s t1 : (τ β[e])) ->
-  Compile j2 (t1' `@ e)
+  Compile t1 j2 (t1' `@ e)
 | appt :
   (j1 : Γ ⊢s t1 : (∀[A]B)) -> -- Γ ⊢ t1 : ∀[A]τ
-  Compile j1 t1' ->
+  Compile t1 j1 t1' ->
   Γ ⊢ τ : A ->
   (j2 : Γ ⊢s t1 : (B β[τ])) ->
-  Compile j2 (t1' `@t τ)
+  Compile t1 j2 (t1' `@t τ)
 | lam :
   (j1 : (.type A :: Γ) ⊢s t1 : τ) ->
   (j2 : Γ ⊢s (.HsLam A t1) : (A -t> τ)) ->
-  Compile j1 t1' ->
-  Compile j2 (`λ[A] t1')
+  (Γ ⊢ (A -t> τ) : ★) ->
+  Compile t1 j1 t1' ->
+  Compile (`λ[A] t1) j2 (`λ[A] t1')
 | letterm :
   Γ ⊢ A : ★ ->
   Γ ⊢ τ : ★ ->
   (j1 : Γ ⊢s t1 : A) ->
-  Compile j1 t1' ->
+  Compile t1 j1 t1' ->
   (j2 : (.term A t1' :: Γ) ⊢s t2 : ([S]τ)) ->
-  Compile j2 t2' ->
+  Compile t2 j2 t2' ->
   (j3 : Γ ⊢s (.HsLet A t1 t2) : τ) ->
-  Compile j3 (.letterm A t1' t2')
+  Compile (.HsLet A t1 t2) j3 (.letterm A t1' t2')
+| ite :
+  Γ ⊢ T : ★ ->
+  Γ ⊢ R : ★ ->
+  StableTypeMatch Γ A R ->
+  PrefixTypeMatch Γ A B T ->
+  ValidHeadVariable R Γ.is_datatype ->
+  HsValidHeadVariable p Γ.is_ctor ->
+  (j1 : Γ ⊢s p : A) ->
+  (j2 : Γ ⊢s s : R) ->
+  (j3 : Γ ⊢s i : B) ->
+  (j4 : Γ ⊢s e : T) ->
+  (j5 : Γ ⊢s .HsIte p s i e : T) ->
+  Compile p j1 p' ->
+  Compile s j2 s' ->
+  Compile i j3 i' ->
+  Compile e j4 e' ->
+  Compile (.HsIte p s i e) j5 (.ite p' s' i' e')
 
-notation:180 "⟅ " j:180 " ⟆=" t:180 => Compile j t
+notation:180 " ⟅ " t:180 " ⟆ " j:180 " ⟶  " t':180 => Compile t j t'
+
+theorem compilation_head_preserving :
+  HsValidHeadVariable p test ->
+  (j : Γ ⊢s p : τ) ->
+  Compile p j p' ->
+  ValidHeadVariable p' test := by
+intro vhv j c;
+induction j;
+all_goals try (cases vhv; case _ h => cases h; case _ w h t => cases h)
+case var x _ _ _ =>
+  cases vhv; case _ w h t =>
+  cases t; case _ f s =>
+  cases f; simp at s;
+  unfold ValidHeadVariable; simp at *;
+  exists x;
+  apply And.intro;
+  { case _ =>
+    cases c;
+    case _ => exists [];
+    case _  e _ _ j c _ =>
+      exists [(.term, e)]; simp; symm;
+      rw[Option.bind_eq_some]; simp;
+      sorry
+    case _ τ _ j c =>
+      exists [(.type, τ)]; simp; symm;
+      rw[Option.bind_eq_some]; simp;
+      sorry }
+  assumption
+
+case implicitArrI j1 j2 ih =>
+  replace ih := ih vhv;
+  sorry
+case implicitArrE => sorry
+case implicitAllI => sorry
+case implicitAllE => sorry
+case app => sorry
 
 theorem compile_type_preserving :
   (j : Γ ⊢s t : τ) ->
-  Compile j t' ->
+  (⟅ t ⟆ j ⟶  t') ->
   Γ ⊢ t' : τ := by
 intro j1 j2;
 induction j2;
-case _ j1 =>
-  cases j1; case _ h =>
-  symm at h;
-  apply Judgment.var; assumption; assumption;
+case _ gt _ =>
+  apply Judgment.var; assumption; symm; assumption
 case _ =>
   apply Judgment.app;
   assumption;
@@ -135,14 +224,24 @@ case appt =>
   assumption;
   assumption;
   rfl
-case _ j2 _  j1  =>
-  cases j2;
+case _ j1 j2 c j3 =>
   apply Judgment.lam;
-  assumption
+  case _ => cases j2; assumption
   assumption
   assumption
 case _ j1 c1 j2 c2 j3 ih1 ih2 =>
   apply Judgment.letterm
+  assumption;
+  assumption;
+  assumption;
+  assumption;
+case _ vhv j1 j2 j3 j4 _ c1 c2 c3 c4 _ _ _ _ =>
+  apply Judgment.ite;
+  assumption;
+  assumption;
+  assumption;
+  assumption;
+  apply compilation_head_preserving vhv; assumption; assumption
   assumption;
   assumption;
   assumption;
